Prove distinction soundness (for now, assuming sensible termination as given)

HML_Strategies_Game.thy
@@ -11,12 +11,15 @@ for
   \<tau> :: \<open>'a\<close> +
 fixes
   strat :: \<open>('s, 'a) c_set_game_node posstrategy\<close> and
-  attacker_winning_region :: \<open>('s, 'a) c_set_game_node set\<close>
+  attacker_winning_region :: \<open>('s, 'a) c_set_game_node set\<close> and
+  attacker_order
+defines
+  \<open>attacker_order \<equiv> {(g', g). c_set_game_moves g g' \<and>
+      g \<in> attacker_winning_region \<and> g' \<in> attacker_winning_region \<and>
+      (player1_position g \<longrightarrow> g' = strat g)}\<^sup>+\<close>
 assumes
   finite_win:
-    \<open>wf {(g, g'). c_set_game_moves g g' \<and>
-      g \<in> attacker_winning_region \<and> g' \<in> attacker_winning_region \<and>
-      (player1_position g \<longrightarrow> g' = strat g)}\<close> and
+    \<open>wf attacker_order\<close> and
   strat_stays_winning:
     \<open>g \<in> attacker_winning_region \<Longrightarrow> player1_position g \<Longrightarrow>
       strat g \<in> attacker_winning_region \<and> c_set_game_moves g (strat g)\<close> and
@@ -35,7 +38,7 @@ function attack_formula :: \<open>('s, 'a) c_set_game_node \<Rightarrow> ('a,'s)
     \<langle>\<tau>\<rangle>\<langle>a\<rangle>(attack_formula (AttackerNode p (dsuccs a Q)))\<close>
 | \<open>attack_formula (DefenderSwapNode p Q) =
     (if Q = {} then HML_true else
-    (HML_weaknor (weak_tau_succs Q) (\<lambda>q. if q \<in> Q then (attack_formula (AttackerNode q {p})) else HML_true )))\<close>
+    (HML_weaknor (weak_tau_succs Q) (\<lambda>q. if q \<in> (weak_tau_succs Q) then (attack_formula (AttackerNode q {p})) else HML_true )))\<close>
   using c_set_game_defender_node.cases
   by (auto, blast)
 
@@ -59,8 +62,11 @@ lemma attack_options:
   assumes
     \<open>(AttackerNode p Q) \<in> attacker_winning_region\<close>
   shows
-    \<open>(\<exists>a p'. attack_formula (AttackerNode p Q) = \<langle>\<tau>\<rangle>\<langle>a\<rangle>(attack_formula (AttackerNode p' (dsuccs a Q))))
-    \<or> (\<exists>p'. attack_formula (AttackerNode p Q) = (HML_weaknor (weak_tau_succs Q) (\<lambda>q. if q \<in> Q then (attack_formula (AttackerNode q {p'})) else HML_true )))
+    \<open>(\<exists>a p'. p =\<rhd>a p' \<and> \<not>tau a \<and> strat (AttackerNode p Q) = (DefenderSimNode a p' Q) \<and>
+      attack_formula (AttackerNode p Q) = \<langle>\<tau>\<rangle>\<langle>a\<rangle>(attack_formula (AttackerNode p' (dsuccs a Q))))
+    \<or> (\<exists>p'. p \<longmapsto>* tau p' \<and> strat (AttackerNode p Q) = (DefenderSwapNode p' Q) \<and>
+      attack_formula (AttackerNode p Q) =
+      (HML_weaknor (weak_tau_succs Q) (\<lambda>q. if q \<in> (weak_tau_succs Q) then (attack_formula (AttackerNode q {p'})) else HML_true )))
     \<or> (Q = {} \<and> attack_formula (AttackerNode p Q) = HML_true)\<close>
 proof -
   from assms have \<open>attack_formula (AttackerNode p Q) = attack_formula (strat (AttackerNode p Q))\<close> by simp
@@ -68,11 +74,12 @@ proof -
     \<open>(\<exists>a p'. (strat (AttackerNode p Q)) = (DefenderSimNode a p' Q) \<and> p  =\<rhd>a p' \<and> \<not>tau a)
     \<or>(\<exists>p'. (strat (AttackerNode p Q)) = (DefenderSwapNode p' Q) \<and> p \<longmapsto>* tau p' )\<close> by blast
   ultimately have 
-    \<open>(\<exists>a p'. (attack_formula (AttackerNode p Q)) = attack_formula (DefenderSimNode a p' Q) \<and> p  =\<rhd>a p' \<and> \<not>tau a)
-    \<or>(\<exists>p'. (attack_formula (AttackerNode p Q)) = attack_formula (DefenderSwapNode p' Q) \<and> p \<longmapsto>* tau p')\<close>
+    \<open>(\<exists>a p'. (strat (AttackerNode p Q)) = (DefenderSimNode a p' Q) \<and>
+      (attack_formula (AttackerNode p Q)) = attack_formula (DefenderSimNode a p' Q) \<and> p  =\<rhd>a p' \<and> \<not>tau a)
+    \<or>(\<exists>p'. (strat (AttackerNode p Q)) = (DefenderSwapNode p' Q) \<and>
+      (attack_formula (AttackerNode p Q)) = attack_formula (DefenderSwapNode p' Q) \<and> p \<longmapsto>* tau p')\<close>
     by metis
-  thus ?thesis unfolding dsuccs_def
-    by (metis attack_formula.simps(2) attack_formula.simps(3) dsuccs_def)
+  thus ?thesis by (standard, force+)
 qed
 
 lemma distinction_soundness:
@@ -85,125 +92,81 @@ lemma distinction_soundness:
     \<open>pQ \<in> attacker_winning_region\<close>
   shows
     \<open>p \<Turnstile> \<phi> \<and> (\<forall>q\<in>Q. \<not> q \<Turnstile> \<phi>)\<close>
-  using finite_win assms(3) unfolding assms(1,2)
-proof (induct)
-  case (less pQ)
-  show ?case proof (cases \<open>attack_formula pQ\<close>)
-qed
-proof (induct rule: attack_formula.induct[of _ \<open>(AttackerNode p Q)\<close>])
-  case (1 p Q)
-  then show ?case
-next
-  case (2 a p Q)
-  then show ?case sorry
-next
-  case (3 p Q)
-  then show ?case sorry
-qed
-
-
-
-lemma distinction_soundness:
-  fixes p Q p0 Q0
-  defines
-    \<open>pQ == AttackerNode p Q\<close>
-  defines
-    \<open>\<phi> == attack_formula pQ\<close>
-  assumes
-    \<open>\<exists>rest. pQ # rest \<in> plays_for_1strategy (strategy_from_positional strat) (AttackerNode p0 Q0)\<close>
-    \<open>player1_winning_strategy (strategy_from_positional strat) pQ\<close>
-    \<open>sound_1strategy (strategy_from_positional strat) pQ\<close>
-  shows
-    \<open>p \<Turnstile> \<phi> \<and> (\<forall>q\<in>Q. \<not> q \<Turnstile> \<phi>)\<close>
-  using assms(3,4,5) unfolding assms(1,2)
-  by (induct arbitrary: p Q rule: attack_formula.induct[of _ \<open>(AttackerNode p Q)\<close>], auto)
-
-lemma distinction_soundness:
-  fixes p Q rest p0 Q0
-  defines
-    \<open>pQ == AttackerNode p Q\<close>
-  defines
-    \<open>\<phi> == attack_formula pQ\<close>
-  assumes
-    \<open>\<exists>rest. pQ # rest \<in> plays_for_1strategy (strategy_from_positional strat) (AttackerNode p0 Q0)\<close>
-    \<open>player1_winning_strategy (strategy_from_positional strat) pQ\<close>
-    \<open>sound_1strategy (strategy_from_positional strat) pQ\<close>
-  shows
-    \<open>p \<Turnstile> \<phi> \<and> (\<forall>q\<in>Q. \<not> q \<Turnstile> \<phi>)\<close>
-  using assms(1,3,4,5) unfolding \<open>\<phi> == attack_formula pQ\<close>
-
-
-  case (1 p' Q')
-  then show ?case sorry
-next
-  case (2 a p Q)
-  then show ?case sorry
-next
-  case (3 p Q)
-  then show ?case sorry
-qed
-  case (1 p' Q')
-  then show ?case sorry
-next
-  case (2 a p' Q')
-  then show ?case by auto
-next
-  case (3 p' Q')
-  then show ?case by auto
-qed
-  case (1)
-  then show ?case sorry
-next
-  case 2
-  then show ?case sorry
-next
-  case 3
-  then show ?case sorry
-qed
-  case (1 p' Q')
-  then show ?case sorry
-next
-  case (2 a p' Q')
-  then show ?case sorry
-next
-  case (3 p' Q')
-  then show ?case sorry
-qed
-
-
-
-  case HML_true
-  hence \<open>False\<close> using attack_options HML_weaknor_def HML_formula.distinct(5)
-    by metis
-  then show ?case ..
-next
-  case (HML_conj Q F)
-  hence \<open>False\<close> using attack_options HML_weaknor_def HML_formula.distinct(9)
-    by metis
-  then show ?case ..
-next
-  case (HML_neg \<phi>)
-  hence \<open>False\<close> using attack_options HML_weaknor_def HML_formula.distinct(11)
-    by metis
-  then show ?case ..
-next
-  case (HML_poss t \<phi>)
-  hence \<open>(\<exists>a p'. attack_formula (AttackerNode p Q) = \<langle>\<tau>\<rangle>\<langle>a\<rangle>(attack_formula (AttackerNode p' (dsuccs a Q))))
-    \<or> (\<exists>p'. attack_formula (AttackerNode p Q) = \<langle>\<tau>\<rangle>(AND (weak_tau_succs Q) (\<lambda>q. HML_neg (attack_formula (AttackerNode q {p'})))))\<close>
-    using attack_options[of p Q] unfolding HML_weaknor_def by blast
-  hence
-    \<open>t = \<tau>\<close>
-    \<open>(\<exists>a p'. \<phi> = \<langle>a\<rangle>(attack_formula (AttackerNode p' (dsuccs a Q))))
-    \<or> (\<exists>p'. \<phi> = (AND (weak_tau_succs Q) (\<lambda>q. HML_neg (attack_formula (AttackerNode q {p'})))))\<close>
-    using \<open>(\<langle>t\<rangle>\<phi>) = attack_formula (AttackerNode p Q)\<close> by auto
-  from this(2) show ?case unfolding \<open>t = \<tau>\<close>
-  proof (rule disjE)
-    assume \<open>\<exists>a p'. \<phi> = \<langle>a\<rangle>attack_formula (AttackerNode p' (dsuccs a Q))\<close>
-    then obtain a p' where phi_def: \<open>\<phi> = \<langle>a\<rangle>attack_formula (AttackerNode p' (dsuccs a Q))\<close> by blast
-    have \<open>player1_winning_strategy (strategy_from_positional strat) (AttackerNode p' (dsuccs a Q))\<close>
-        \<open>sound_1strategy (strategy_from_positional strat) (AttackerNode p' (dsuccs a Q))\<close> sorry
-    with HML_poss(1) phi_def have \<open>p' \<Turnstile> \<phi> \<and> (\<forall>q\<in>(dsuccs a Q). \<not> q \<Turnstile> \<phi>)\<close>
-    show \<open>(p \<Turnstile> (\<langle>\<tau>\<rangle>\<phi>)) \<and> (\<forall>q\<in>Q. \<not> (q \<Turnstile> (\<langle>\<tau>\<rangle>\<phi>)))\<close> sorry
+  using finite_win assms
+proof (induct arbitrary: p Q \<phi>)
+  case (less p Q)
+  from attack_options[OF this(2)] show ?case
+  proof
+    assume \<open>\<exists>a p'. p =\<rhd> a  p' \<and> \<not> tau a \<and> strat (AttackerNode p Q) = DefenderSimNode a p' Q \<and>
+      attack_formula (AttackerNode p Q) = \<langle>\<tau>\<rangle>\<langle>a\<rangle>attack_formula (AttackerNode p' (dsuccs a Q))\<close>
+    then obtain a p' where case_assms:
+      \<open>p =\<rhd> a  p' \<and> \<not> tau a\<close>
+      \<open>strat (AttackerNode p Q) = DefenderSimNode a p' Q\<close>
+      \<open>attack_formula (AttackerNode p Q) = \<langle>\<tau>\<rangle>\<langle>a\<rangle>attack_formula (AttackerNode p' (dsuccs a Q))\<close> by blast
+    hence moves:
+      \<open>c_set_game_moves (AttackerNode p Q) (DefenderSimNode a p' Q)\<close>
+      \<open>c_set_game_moves (DefenderSimNode a p' Q) (AttackerNode p' (dsuccs a Q))\<close> by auto
+    with case_assms less(2) defender_keeps_losing strat_stays_winning have all_winning:
+      \<open>(AttackerNode p' (dsuccs a Q)) \<in> attacker_winning_region\<close>
+      \<open>(DefenderSimNode a p' Q) \<in> attacker_winning_region\<close>
+        by (metis c_set_game_defender_node.simps(2), force)
+    with case_assms moves less(2) have
+      \<open>(AttackerNode p' (dsuccs a Q), DefenderSimNode a p' Q) \<in> attacker_order\<close>
+      \<open>(DefenderSimNode a p' Q, AttackerNode p Q) \<in> attacker_order\<close>
+      unfolding attacker_order_def by (simp add: r_into_trancl')+
+    hence \<open>(AttackerNode p' (dsuccs a Q), AttackerNode p Q) \<in> attacker_order\<close>
+      unfolding attacker_order_def by auto
+    with less.hyps all_winning(1) have
+      \<open>p' \<Turnstile> attack_formula (AttackerNode p' (dsuccs a Q)) \<and> (\<forall>q\<in>(dsuccs a Q). \<not> q \<Turnstile> attack_formula (AttackerNode p' (dsuccs a Q)))\<close>
+      by blast
+    with case_assms have
+      \<open>p \<Turnstile> \<langle>\<tau>\<rangle>\<langle>a\<rangle>attack_formula (AttackerNode p' (dsuccs a Q))\<close>
+      \<open>\<forall>q\<in>Q. \<not>q \<Turnstile> \<langle>\<tau>\<rangle>\<langle>a\<rangle>attack_formula (AttackerNode p' (dsuccs a Q))\<close>
+      unfolding dsuccs_def by (auto, blast+)
+    thus ?case unfolding case_assms by blast
+  next
+    assume \<open>(\<exists>p'. p \<longmapsto>* tau  p' \<and> strat (AttackerNode p Q) = DefenderSwapNode p' Q \<and>
+        attack_formula (AttackerNode p Q) = HML_weaknor (weak_tau_succs Q) (\<lambda>q. if q \<in> (weak_tau_succs Q) then attack_formula (AttackerNode q {p'}) else HML_true)) \<or>
+      Q = {} \<and> attack_formula (AttackerNode p Q) = HML_true\<close>
+    thus ?case
+    proof
+      assume \<open>\<exists>p'. p \<longmapsto>* tau  p' \<and> strat (AttackerNode p Q) = DefenderSwapNode p' Q \<and>
+        attack_formula (AttackerNode p Q) = HML_weaknor (weak_tau_succs Q) (\<lambda>q. if q \<in> (weak_tau_succs Q) then attack_formula (AttackerNode q {p'}) else HML_true)\<close>
+      then obtain p' where case_assms:
+        \<open>p \<longmapsto>* tau  p'\<close>
+        \<open>strat (AttackerNode p Q) = DefenderSwapNode p' Q\<close>
+        \<open>attack_formula (AttackerNode p Q) = HML_weaknor (weak_tau_succs Q) (\<lambda>q. if q \<in> (weak_tau_succs Q) then attack_formula (AttackerNode q {p'}) else HML_true)\<close>
+        by blast
+      from case_assms have moves:
+        \<open>c_set_game_moves (AttackerNode p Q) (DefenderSwapNode p' Q)\<close>
+        \<open>\<forall>q'\<in>(weak_tau_succs Q). c_set_game_moves (DefenderSwapNode p' Q) (AttackerNode q' {p'})\<close> by auto
+      with case_assms less(2) defender_keeps_losing strat_stays_winning have all_winning:
+        \<open>(DefenderSwapNode p' Q) \<in> attacker_winning_region\<close>
+        \<open>\<forall>q'\<in>(weak_tau_succs Q). (AttackerNode q' {p'}) \<in> attacker_winning_region\<close>
+        by (metis, metis c_set_game_defender_node.simps(1,3))
+      with case_assms moves less(2) have
+        \<open>\<forall>q'\<in> weak_tau_succs Q. (AttackerNode q' {p'}, DefenderSwapNode p' Q) \<in> attacker_order\<close>
+        \<open>(DefenderSwapNode p' Q, AttackerNode p Q) \<in> attacker_order\<close>
+        unfolding attacker_order_def by (simp add: r_into_trancl')+
+      hence \<open>\<forall>q'\<in> weak_tau_succs Q. (AttackerNode q' {p'}, AttackerNode p Q) \<in> attacker_order\<close>
+        unfolding attacker_order_def by auto
+      with less.hyps all_winning have
+        \<open>\<forall>q'\<in> weak_tau_succs Q. q' \<Turnstile> attack_formula (AttackerNode q' {p'}) \<and> \<not> p' \<Turnstile> attack_formula (AttackerNode q' {p'})\<close>
+        by blast
+      with case_assms have
+        \<open>p' \<Turnstile> HML_conj (weak_tau_succs Q) (\<lambda>q'. HML_neg (attack_formula (AttackerNode q' {p'})))\<close>
+        \<open>\<forall>q'\<in> weak_tau_succs Q. \<not> q' \<Turnstile> HML_conj (weak_tau_succs Q) (\<lambda>qq'. HML_neg (attack_formula (AttackerNode qq' {p'})))\<close>
+        by (simp, fastforce)
+      with case_assms have
+        \<open>p \<Turnstile>  HML_weaknor (weak_tau_succs Q) (\<lambda>q. if q \<in> (weak_tau_succs Q) then attack_formula (AttackerNode q {p'}) else HML_true)\<close>
+        \<open>\<forall>q\<in>Q. \<not>q \<Turnstile>  HML_weaknor (weak_tau_succs Q) (\<lambda>q. if q \<in> (weak_tau_succs Q) then attack_formula (AttackerNode q {p'}) else HML_true)\<close>
+        unfolding weak_tau_succs_def HML_weaknor_def
+        using conj_only_depends_on_indexset by (auto, force, fastforce)
+      thus ?case unfolding case_assms by blast
+    next
+      assume \<open>Q = {} \<and> attack_formula (AttackerNode p Q) = HML_true\<close>
+      thus ?case by auto
+    qed
   qed
 qed
 
